src/high/modalities/if_rec.v
@@ -1,0 +1,163 @@
+From iris.proofmode Require Import tactics.
+From iris.bi Require Import bi.
+From iris.bi Require Import derived_laws.
+From iris.base_logic Require Import iprop.
+
+From self.base Require Import primitive_laws wpr_lifting.
+From self.high Require Import dprop resources modalities or_lost monpred_simpl.
+
+(* The predicate [P] holds for [ℓ] or [ℓ] has been lost. *)
+Definition if_rec `{nvmBaseFixedG Σ, nvmBaseDeltaG Σ}
+           (ℓ : loc) (P : dProp Σ) : dProp Σ :=
+  ∀ (CV : view),
+    ⌜ is_Some (CV !! ℓ) ⌝ -∗ ⎡ crashed_at CV ⎤ -∗ ⎡ persisted_loc ℓ 0 ⎤ -∗ P.
+
+(* alt
+  P ∨ (∃ CV, ⎡crashed_at CV⎤ ∗ ⌜ℓ ∉ dom (gset _) CV⌝ )
+ *)
+
+Class IntoIfRec `{nvmBaseFixedG Σ, nvmBaseDeltaG Σ} ℓ (P : dProp Σ) (Q : dProp Σ) :=
+  into_if_rec : P ⊢ if_rec ℓ Q.
+Global Arguments IntoIfRec {_} {_} {_} _ _%I _%I.
+Global Arguments into_if_rec {_} _ _%I _%I.
+Global Hint Mode IntoIfRec ! ! ! + + -  : typeclass_instances.
+
+Section if_rec.
+  Context `{nvmBaseFixedG Σ, nvmBaseDeltaG Σ}.
+
+  Local Ltac ifRecIntro := iIntros (CV) "%look #crashed #pers".
+
+  Lemma if_rec_intro ℓ P : P -∗ if_rec ℓ P.
+  Proof. iIntros "P". ifRecIntro. done. Qed.
+
+  Lemma if_rec_and ℓ P Q : if_rec ℓ (P ∧ Q) ⊣⊢ if_rec ℓ P ∧ if_rec ℓ Q.
+  Proof.
+    iSplit.
+    - iIntros "H".
+      iSplit; ifRecIntro.
+      * iDestruct ("H" $! CV with "[//] crashed [$]") as "[$ _]".
+      * iDestruct ("H" $! CV with "[//] crashed [$]") as "[_ $]".
+    - iIntros "H". ifRecIntro.
+      iSplit.
+      * iDestruct "H" as "[H _]". iApply "H"; done.
+      * iDestruct "H" as "[_ H]". iApply "H"; done.
+  Qed.
+
+  Lemma if_rec_sep ℓ (P Q : dProp Σ) :
+    if_rec ℓ P ∗ if_rec ℓ Q -∗ if_rec ℓ (P ∗ Q)%I.
+  Proof.
+    iIntros "[P Q]". ifRecIntro.
+    iDestruct ("P" $! CV with "[//] crashed [$]") as "$".
+    iDestruct ("Q" $! CV with "[//] crashed [$]") as "$".
+  Qed.
+
+  Lemma if_rec_mono ℓ (P Q : dProp Σ) :
+    (P -∗ Q) → if_rec ℓ P -∗ if_rec ℓ Q.
+  Proof.
+    rewrite /if_rec.
+    intros pToQ.
+    iIntros "P". ifRecIntro.
+    iApply pToQ.
+    iApply "P"; done.
+  Qed.
+
+  Lemma if_rec_emp ℓ : (emp : dProp Σ) ⊢ if_rec ℓ emp.
+  Proof. iIntros "_". ifRecIntro. done. Qed.
+
+  Lemma if_rec_intuitionistically_2 ℓ P : □ (if_rec ℓ P) ⊢ if_rec ℓ (□ P).
+  Proof. iIntros "#P". ifRecIntro. iModIntro. iApply "P"; done. Qed.
+
+  Lemma modality_if_rec_mixin ℓ :
+    modality_mixin (@if_rec Σ _ _ ℓ)
+      (MIEnvTransform (IntoIfRec ℓ)) (MIEnvTransform (IntoIfRec ℓ)).
+  Proof.
+    split; simpl; split_and?;
+      eauto using bi.equiv_entails_1_2, if_rec_and, if_rec_emp,
+        if_rec_mono, if_rec_sep.
+    intros P Q. rewrite /IntoIfRec=> ->.
+    by rewrite if_rec_intuitionistically_2.
+  Qed.
+
+  Definition modality_if_rec ℓ :=
+    Modality _ (modality_if_rec_mixin ℓ).
+
+  Global Instance from_modal_if_rec P ℓ :
+    FromModal True (modality_if_rec ℓ) (if_rec ℓ P) (if_rec ℓ P) P.
+  Proof. by rewrite /FromModal. Qed.
+
+  Global Instance if_rec_mono' ℓ : Proper ((⊢) ==> (⊢)) (if_rec (Σ := Σ) ℓ).
+  Proof. intros P Q. apply if_rec_mono. Qed.
+
+  Global Instance if_rec_objective ℓ `{!Objective P} : Objective (if_rec ℓ P).
+  Proof.
+    iIntros (TV1 ?) "P".
+    iIntros (CV ?? look ??) "crashed".
+    iIntros (??) "pers".
+    iSpecialize ("P" $! CV look).
+    monPred_simpl. iSpecialize ("P" $! TV1 with "[//] crashed").
+    monPred_simpl. iSpecialize ("P" $! TV1 with "[//] pers").
+    iApply objective_at.
+    iApply "P".
+  Qed.
+
+  Lemma if_rec_get CV ℓ P :
+    is_Some (CV !! ℓ) → ⎡ crashed_at CV ⎤ -∗ ⎡ persisted_loc ℓ 0 ⎤ -∗ if_rec ℓ P -∗ P.
+  Proof. iIntros ([[t] look]) "#? #? H". iApply "H"; naive_solver. Qed.
+
+  (* Lemma if_rec_with_t_get CV ℓ t P : *)
+  (*   CV !! ℓ = Some (MaxNat t) → ⎡ crashed_at CV ⎤ -∗ if_rec_with_t ℓ P -∗ P t. *)
+  (* Proof. *)
+  (*   rewrite /if_rec_with_t. *)
+  (*   iIntros (look) "crash (%CV' & crash' & [(%t' & %look' & P)|%look'])"; *)
+  (*   iDestruct (crashed_at_agree with "crash crash'") as %<-. *)
+  (*   - simplify_eq. iFrame "P". *)
+  (*   - congruence. *)
+  (* Qed. *)
+
+  Lemma if_rec_is_rec ℓ :
+    ⊢ if_rec ℓ (∃ CV,
+      ⌜ is_Some (CV !! ℓ) ⌝ ∗ ⎡ crashed_at CV ⎤ ∗ ⎡ persisted_loc ℓ 0 ⎤).
+  Proof. ifRecIntro. iExists CV. iFrame "#%". Qed.
+
+  Lemma if_rec_is_persisted ℓ :
+    ⊢ if_rec ℓ ⎡ persisted_loc ℓ 0 ⎤.
+  Proof. ifRecIntro. iFrame "#". Qed.
+
+  Lemma or_lost_if_rec_embed ℓ P TV :
+    or_lost_post_crash_no_t ℓ P -∗ (if_rec ℓ ⎡ P ⎤) TV.
+  Proof.
+    iDestruct 1 as (CV) "[crash disj]".
+    iIntros (CV'). monPred_simpl. iIntros (??). monPred_simpl.
+    iIntros ([??] ??). monPred_simpl. iIntros "crashed" (??) "pers".
+    iDestruct (crashed_at_agree with "crash crashed") as %->.
+    iDestruct "disj" as "[(%t & %look & [_ $]) | %]". congruence.
+  Qed.
+
+  Lemma if_rec_or_lost_with_t ℓ P :
+    or_lost_with_t ℓ P -∗ if_rec ℓ (∃ t, P t).
+  Proof.
+    iIntros "(%CV' & #crashed' & disj)".
+    ifRecIntro. destruct look as [??].
+    iDestruct (crashed_at_agree with "crashed crashed'") as %<-.
+    iDestruct "disj" as "[(% & % & #per & P) | %lost]"; last congruence.
+    iExists t. iFrame "P".
+  Qed.
+
+  Global Instance into_if_rec_intro ℓ P : IntoIfRec ℓ P P := if_rec_intro ℓ P.
+
+  Global Instance if_rec_into_if_rec ℓ P : IntoIfRec ℓ (if_rec ℓ P) P.
+  Proof. done. Qed.
+
+  (* Global Instance into_if_rec_or_lost_with_t ℓ P : *)
+  (*   IntoIfRec ℓ (or_lost_with_t ℓ P) (∃ t, P t). *)
+  (* Proof. *)
+  (*   rewrite /IntoIfRec. *)
+  (*   iIntros "H". *)
+  (*   ifRecIntro. destruct look as [[?]?]. *)
+  (*   iDestruct (or_lost_with_t_get with "[$] H") as "H"; first done. *)
+  (*   naive_solver. *)
+  (* Qed. *)
+
+End if_rec.
+
+Opaque if_rec.
